

$$SC(\Delta e) = \sum_e \left( \frac{1}{\alpha_e} \Delta e^2 - \Delta e \beta_e \right) \quad \text{w/ } \Delta e = \lambda_n - \lambda_m$$

$$\frac{d}{d\beta_k} SC(\Delta e) = \underbrace{\sum_e \left( \frac{2}{\alpha_e} \Delta e \Delta e' \right)}_A - \underbrace{\sum_e \left( \frac{\beta_e}{\alpha_e} \Delta e' \right)}_B - \underbrace{\frac{1}{\alpha_k} \Delta k}_C$$

claim:  $\frac{d}{d\beta_k} SC(\Delta e) = \text{const} \Rightarrow SC(\Delta e)$  linear in  $\beta_e$

wx:

- $\vec{\lambda} = -C\vec{\beta} + D\vec{P} \quad \text{w/ } M^{-1} = \begin{pmatrix} A & B \\ C & D \end{pmatrix}$
- $\frac{d}{d\beta_e} \vec{\lambda} = -C$

from  $\vec{x} = M\vec{y}$

$$\Rightarrow \lambda_n = -\sum_e C_{ne} \beta_e + \sum_j D_{nj} P_j$$

$$\frac{\partial}{\partial \beta_e} \lambda_n = -C_{ne}$$

Different C!

This is true but not proven, yet.

proof:  $\frac{d}{d\beta_k} SC(\Delta e) = A - B - C = -B + C$

$$B = \sum_e \frac{\beta_e}{\alpha_e} (\lambda_n' - \lambda_m') = \sum_e \frac{\beta_e}{\alpha_e} (C_{ne} - C_{me})$$

Unter fehlt ein  $\alpha$ .

$$C = \frac{1}{\alpha_n} \Delta e = \frac{1}{\alpha_{ab}} (\lambda_a - \lambda_b) = \left( \sum_e C_{ae} \beta_e + \sum_j D_{aj} P_j + \sum_e C_{be} \beta_e - \sum_j D_{bj} P_j \right) \frac{1}{\alpha_{ab}}$$

$$= \left( \sum_e (C_{be} - C_{ae}) \beta_e + \sum_j (D_{aj} - D_{bj}) P_j \right) \frac{1}{\alpha_{ab}}$$

$$\Rightarrow \frac{d}{d\beta_n} SC(\Delta e) = C - B = \frac{1}{\alpha_{ab}} \sum_j (D_{aj} - D_{bj}) P_j$$